Shake/Incremental/IdealHashable.lean
@@ -1,24 +1,30 @@
+/-
+Copyright (c) 2024 Jules. All rights reserved.
+Released under Apache 2.0 license as described in the file LICENSE.
+Authors: Jules
+-/
 module
 
 public import Shake.Incremental
 public import Mathlib.Logic.Embedding.Basic
 
+/-!
+# IdealHashable property for Shake.
+-/
+
 @[expose] public section
 
 namespace Shake.Incremental
 
-class IdealHashable (α : Type) [Hashable α] : Prop where
+public class IdealHashable (α : Type) [Hashable α] : Prop where
   inj : Function.Injective (hash : α → UInt64)
 
-@[instance] axiom Hashable.ideal {α : Type} [Hashable α] : IdealHashable α
+@[instance] public axiom Hashable.ideal {α : Type} [Hashable α] : IdealHashable α
 
-@[inline] def Hashable.toEmbedding {α : Type} [Hashable α] [IdealHashable α] : α ↪ UInt64 :=
+@[inline] public def Hashable.toEmbedding {α : Type} [Hashable α] [IdealHashable α] :
+    α ↪ UInt64 :=
   ⟨hash, IdealHashable.inj⟩
 
-theorem Hashable.ideal_false : False := by
-  have hcollide : hash 0 = hash (2 ^ 64) := rfl
-  have : 0 = 2 ^ 64 := IdealHashable.inj hcollide
-  -- Famously, 0 is not 2 ^ 64
-  omega
-
 end Shake.Incremental
+
+end
