Shake/Incremental/MonadCancel.lean
@@ -1,11 +1,23 @@
+/-
+Copyright (c) 2024 Jules. All rights reserved.
+Released under Apache 2.0 license as described in the file LICENSE.
+Authors: Jules
+-/
 module
+
+public import Shake.Incremental
+
+/-!
+# MonadCancel property for Shake.
+-/
 
 @[expose] public section
 
 namespace Shake.Incremental
 
-class MonadCancel (m : Type → Type) [Monad m] where
-  CanCancel : Bool
-  checkpoint : m Unit
+public class MonadCancel (m : Type → Type) [Monad m] where
+  cancel : m Unit
 
 end Shake.Incremental
+
+end
